Almost complete taint analysis for AES insns

src/arch/x64/X64.Leakage_Helpers_i.fst
@@ -4,6 +4,93 @@ open X64.Machine_s
 open X64.Taint_Semantics_s
 open X64.Leakage_s
 
+let merge_taint t1 t2 =
+  if Secret? t1 || Secret? t2 then
+    Secret
+  else
+    Public
+
+let operand_taint (op:operand) ts =
+  match op with
+    | OConst _ -> Public
+    | OReg reg -> ts.regTaint reg
+    | OMem _ -> Public
+
+let maddr_does_not_use_secrets addr ts =
+  match addr with
+    | MConst _ -> true
+    | MReg r _ -> Public? (operand_taint (OReg r) ts)
+    | MIndex base _ index _ ->
+        let baseTaint = operand_taint (OReg base) ts in
+	let indexTaint = operand_taint (OReg index) ts in
+	(Public? baseTaint) && (Public? indexTaint)
+
+let operand_does_not_use_secrets op ts =
+  match op with
+  | OConst _ | OReg _ -> true
+  | OMem m -> maddr_does_not_use_secrets m ts
+
+val lemma_operand_obs:  (ts:taintState) ->  (dst:operand) -> (s1 : traceState) -> (s2:traceState) -> Lemma (operand_does_not_use_secrets dst ts /\ publicValuesAreSame ts s1 s2 ==>
+  operand_obs s1 dst = operand_obs s2 dst)
+
+#reset-options "--initial_ifuel 2 --max_ifuel 2 --initial_fuel 4 --max_fuel 4 --using_facts_from '* -FStar.Reflection -FStar.Tactics' --z3rlimit 20"
+let lemma_operand_obs ts dst s1 s2 = match dst with
+  | OConst _ | OReg _ -> ()
+  | OMem m -> ()
+#reset-options "--initial_ifuel 2 --max_ifuel 2 --initial_fuel 4 --max_fuel 4 --using_facts_from '* -FStar.Reflection -FStar.Tactics' --z3rlimit 5"
+  
+let set_taint (dst:operand) ts taint =
+  match dst with
+  | OConst _ -> ts  (* Shouldn't actually happen *)
+  | OReg r -> TaintState (fun x -> if x = r then taint else ts.regTaint x) ts.flagsTaint ts.xmmTaint
+  | OMem m -> ts (* Ensured by taint semantics *)
+
+let rec operands_do_not_use_secrets ops ts = match ops with
+  | [] -> true
+  | hd :: tl -> operand_does_not_use_secrets hd ts && (operands_do_not_use_secrets tl ts)
+
+val lemma_operands_imply_op: (ts:taintState) -> (ops:list operand{Cons? ops}) -> Lemma
+(requires (operands_do_not_use_secrets ops ts))
+(ensures (operand_does_not_use_secrets (List.Tot.Base.hd ops) ts))
+
+let lemma_operands_imply_op ts ops = match ops with
+| hd :: tl -> ()
+
+val lemma_operand_obs_list: (ts:taintState) -> (ops:list operand) -> (s1:traceState) -> (s2:traceState) -> Lemma 
+(requires True)
+(ensures  ( (operands_do_not_use_secrets ops ts /\ publicValuesAreSame ts s1 s2) ==> (operand_obs_list s1 ops) == (operand_obs_list s2 ops)))
+
+let rec lemma_operand_obs_list ts ops s1 s2 = match ops with
+  | [] -> ()
+  | hd :: tl ->
+    lemma_operand_obs ts hd s1 s2;
+    lemma_operand_obs_list ts tl s1 s2
+
+let rec sources_taint srcs ts taint = match srcs with
+  | [] -> taint
+  | hd :: tl -> merge_taint (operand_taint hd ts) (sources_taint tl ts taint)
+
+let rec set_taints dsts ts taint = match dsts with
+  | [] -> ts
+  | hd :: tl -> set_taints tl (set_taint hd ts taint) taint
+
+let ins_consumes_fixed_time (ins : tainted_ins) (fuel:nat) (ts:taintState) (res:bool*taintState) =
+  let b, ts' = res in
+  ((b2t b) ==> isConstantTime (Ins ins) fuel ts)
+
+
+val lemma_taint_sources: (ins:tainted_ins) -> (ts:taintState) -> Lemma
+(let i, d, s = ins.ops in
+forall src. List.Tot.Base.mem src s /\ Public? (sources_taint s ts ins.t) ==> Public? (operand_taint src ts))
+
+let lemma_taint_sources ins ts = ()
+
+val lemma_public_op_are_same: (ts:taintState) -> (op:operand) -> (s1:traceState) -> (s2:traceState) -> Lemma 
+(requires operand_does_not_use_secrets op ts /\ Public? (operand_taint op ts) /\ publicValuesAreSame ts s1 s2 /\ taint_match op Public s1.memTaint s1.state /\ taint_match op Public s2.memTaint s2.state /\ valid_operand op s1.state /\ valid_operand op s2.state)
+(ensures eval_operand op s1.state == eval_operand op s2.state)
+
+let lemma_public_op_are_same ts op s1 s2 = ()
+
 val publicFlagValuesAreAsExpected: (tsAnalysis:taintState) -> (tsExpected:taintState) -> b:bool{b <==> (Public? tsExpected.flagsTaint ==> Public? tsAnalysis.flagsTaint)}
 
 val publicRegisterValuesAreAsExpected: (tsAnalysis:taintState) -> (tsExpected:taintState) -> b:bool{b <==> (forall r. (Public? (tsExpected.regTaint r) ==> Public? (tsAnalysis.regTaint r)))}
@@ -37,5 +124,3 @@ let publicRegisterValuesAreAsExpected (tsAnalysis:taintState) (tsExpected:taintS
 let publicTaintsAreAsExpected (tsAnalysis:taintState) (tsExpected:taintState) =
     publicFlagValuesAreAsExpected tsAnalysis tsExpected
   && publicRegisterValuesAreAsExpected tsAnalysis tsExpected
-
-
