src/arch/x64/X64.Leakage_Ins_i.fst
@@ -9,93 +9,9 @@ open FStar.Tactics
 
 #reset-options "--initial_ifuel 2 --max_ifuel 2 --initial_fuel 4 --max_fuel 4 --using_facts_from '* -FStar.Reflection -FStar.Tactics'"
 
-let merge_taint t1 t2 =
-  if Secret? t1 || Secret? t2 then
-    Secret
-  else
-    Public
 
-let operand_taint (op:operand) ts =
-  match op with
-    | OConst _ -> Public
-    | OReg reg -> ts.regTaint reg
-    | OMem _ -> Public
-
-let maddr_does_not_use_secrets addr ts =
-  match addr with
-    | MConst _ -> true
-    | MReg r _ -> Public? (operand_taint (OReg r) ts)
-    | MIndex base _ index _ ->
-        let baseTaint = operand_taint (OReg base) ts in
-	let indexTaint = operand_taint (OReg index) ts in
-	(Public? baseTaint) && (Public? indexTaint)
-
-let operand_does_not_use_secrets op ts =
-  match op with
-  | OConst _ | OReg _ -> true
-  | OMem m -> maddr_does_not_use_secrets m ts
-
-val lemma_operand_obs:  (ts:taintState) ->  (dst:operand) -> (s1 : traceState) -> (s2:traceState) -> Lemma
- (requires (operand_does_not_use_secrets dst ts) /\ publicValuesAreSame ts s1 s2)
-(ensures (operand_obs s1 dst) = (operand_obs s2 dst))
-
-#reset-options "--initial_ifuel 2 --max_ifuel 2 --initial_fuel 4 --max_fuel 4 --using_facts_from '* -FStar.Reflection -FStar.Tactics' --z3rlimit 20"
-let lemma_operand_obs ts dst s1 s2 = match dst with
-  | OConst _ | OReg _ -> ()
-  | OMem m -> ()
-#reset-options "--initial_ifuel 2 --max_ifuel 2 --initial_fuel 4 --max_fuel 4 --using_facts_from '* -FStar.Reflection -FStar.Tactics' --z3rlimit 5"
-  
-let set_taint (dst:operand) ts taint =
-  match dst with
-  | OConst _ -> ts  (* Shouldn't actually happen *)
-  | OReg r -> TaintState (fun x -> if x = r then taint else ts.regTaint x) ts.flagsTaint
-  | OMem m -> ts (* Ensured by taint semantics *)
-
-let rec operands_do_not_use_secrets ops ts = match ops with
-  | [] -> true
-  | hd :: tl -> operand_does_not_use_secrets hd ts && (operands_do_not_use_secrets tl ts)
-
-val lemma_operands_imply_op: (ts:taintState) -> (ops:list operand{Cons? ops}) -> Lemma
-(requires (operands_do_not_use_secrets ops ts))
-(ensures (operand_does_not_use_secrets (List.Tot.Base.hd ops) ts))
-
-let lemma_operands_imply_op ts ops = match ops with
-| hd :: tl -> ()
-
-val lemma_operand_obs_list: (ts:taintState) -> (ops:list operand) -> (s1:traceState) -> (s2:traceState) -> Lemma 
-(requires (operands_do_not_use_secrets ops ts /\ publicValuesAreSame ts s1 s2))
-(ensures  (operand_obs_list s1 ops) == (operand_obs_list s2 ops))
-
-let rec lemma_operand_obs_list ts ops s1 s2 = match ops with
-  | [] -> ()
-  | hd :: tl -> assert (operand_does_not_use_secrets hd ts); assert_by_tactic (operand_obs s1 hd = operand_obs s2 hd) (apply_lemma (quote (lemma_operand_obs ts))); lemma_operand_obs_list ts tl s1 s2
-
-let rec sources_taint srcs ts taint = match srcs with
-  | [] -> taint
-  | hd :: tl -> merge_taint (operand_taint hd ts) (sources_taint tl ts taint)
-
-let rec set_taints dsts ts taint = match dsts with
-  | [] -> ts
-  | hd :: tl -> set_taints tl (set_taint hd ts taint) taint
-
-let ins_consumes_fixed_time (ins : tainted_ins) (fuel:nat) (ts:taintState) (res:bool*taintState) =
-  let b, ts' = res in
-  ((b2t b) ==> isConstantTime (Ins ins) fuel ts)
-
-val check_if_ins_consumes_fixed_time: (ins:tainted_ins) -> (fuel:nat) -> (ts:taintState) -> (res:(bool*taintState){ins_consumes_fixed_time ins fuel ts res})
+val check_if_ins_consumes_fixed_time: (ins:tainted_ins{not (is_xmm_ins ins)}) -> (fuel:nat) -> (ts:taintState) -> (res:(bool*taintState){ins_consumes_fixed_time ins fuel ts res})
 #reset-options "--initial_ifuel 2 --max_ifuel 2 --initial_fuel 4 --max_fuel 4 --using_facts_from '* -FStar.Reflection -FStar.Tactics' --z3rlimit 30"
-
-val lemma_taint_sources: (ins:tainted_ins) -> (ts:taintState) -> Lemma
-(let i, d, s = ins.ops in
-forall src. List.Tot.Base.mem src s /\ Public? (sources_taint s ts ins.t) ==> Public? (operand_taint src ts))
-
-let lemma_taint_sources ins ts = ()
-
-val lemma_public_op_are_same: (ts:taintState) -> (op:operand) -> (s1:traceState) -> (s2:traceState) -> Lemma 
-(requires operand_does_not_use_secrets op ts /\ Public? (operand_taint op ts) /\ publicValuesAreSame ts s1 s2 /\ taint_match op Public s1.memTaint s1.state /\ taint_match op Public s2.memTaint s2.state /\ valid_operand op s1.state /\ valid_operand op s2.state)
-(ensures eval_operand op s1.state == eval_operand op s2.state)
-
-let lemma_public_op_are_same ts op s1 s2 = ()
 
 let check_if_ins_consumes_fixed_time ins fuel ts =
   let i, dsts, srcs = ins.ops in
@@ -103,10 +19,8 @@ let check_if_ins_consumes_fixed_time ins fuel ts =
   let ftDsts = operands_do_not_use_secrets dsts ts in
   let fixedTime = ftSrcs && ftDsts in
 
-  assert_by_tactic (forall s1 s2. {:pattern (publicValuesAreSame ts s1 s2)} (operands_do_not_use_secrets dsts ts /\ publicValuesAreSame ts s1 s2) ==>
-    (operand_obs_list s1 dsts) == (operand_obs_list s2 dsts)) (s1 <-- forall_intro; s2 <-- forall_intro; h <-- implies_intro; apply_lemma (quote (lemma_operand_obs_list ts dsts))); 
-
-  assert_by_tactic (forall s1 s2. (operands_do_not_use_secrets srcs ts /\ publicValuesAreSame ts s1 s2) ==> (operand_obs_list s1 srcs) == (operand_obs_list s2 srcs)) (s1 <-- forall_intro; s2 <-- forall_intro; h <-- implies_intro; apply_lemma (quote (lemma_operand_obs_list ts srcs)));
+  Classical.forall_intro_2 (fun x y -> lemma_operand_obs_list ts dsts x y);
+  Classical.forall_intro_2 (lemma_operand_obs_list ts srcs);
   assert (fixedTime ==> (isConstantTime (Ins ins) fuel ts));
   let taint = sources_taint srcs ts ins.t in
   let taint = if AddCarry64? i then merge_taint taint ts.flagsTaint else taint in
@@ -118,28 +32,24 @@ let check_if_ins_consumes_fixed_time ins fuel ts =
 	| OReg r -> fixedTime, ts'
 	| OMem m -> (fixedTime && (not (Secret? taint && Public? (operand_taint (OMem m) ts)))), ts'
     end
-    | Mul64 _ -> fixedTime, (TaintState ts'.regTaint Secret)
+    | Mul64 _ -> fixedTime, (TaintState ts'.regTaint Secret ts'.xmmTaint)
     | Xor64 dst src -> 
         (* Special case for Xor : xor-ing an operand with itself erases secret data *)
         if dst = src then
 	  let ts' = set_taint dst ts' Public in
-	  fixedTime, TaintState ts'.regTaint Secret
+	  fixedTime, TaintState ts'.regTaint Secret ts'.xmmTaint
         else begin match dst with
 	  | OConst _ -> false, ts (* Should not happen *)
-	  | OReg r -> fixedTime, (TaintState ts'.regTaint Secret)
-	  | OMem m -> (fixedTime && (not (Secret? taint && Public? (operand_taint (OMem m) ts)))), (TaintState ts'.regTaint Secret)
+	  | OReg r -> fixedTime, (TaintState ts'.regTaint Secret ts'.xmmTaint)
+	  | OMem m -> (fixedTime && (not (Secret? taint && Public? (operand_taint (OMem m) ts)))), (TaintState ts'.regTaint Secret ts'.xmmTaint)
         end
     | _ -> 
       match dsts with
 	| [OConst _] -> false, ts (* Should not happen *)
-	| [OReg r] -> fixedTime, (TaintState ts'.regTaint Secret)
-	| [OMem m] ->  (fixedTime && (not (Secret? taint && Public? (operand_taint (OMem m) ts)))), (TaintState ts'.regTaint Secret)
+	| [OReg r] -> fixedTime, (TaintState ts'.regTaint Secret ts'.xmmTaint)
+	| [OMem m] ->  (fixedTime && (not (Secret? taint && Public? (operand_taint (OMem m) ts)))), (TaintState ts'.regTaint Secret ts'.xmmTaint)
   in
   b, ts'
-
-//val lemma_public_flags_same: (ts:taintState) -> (fuel:nat) -> (ins:tainted_ins) -> Lemma (forall s1 s2. publicFlagValuesAreSame ts s1 s2 ==> publicFlagValuesAreSame (snd (check_if_ins_consumes_fixed_time ins fuel ts)) (taint_eval_ins ins s1) (taint_eval_ins ins s2))
-
-//let lemma_public_flags_same ts fuel ins = ()
 
 val lemma_mov_same_public: (ts:taintState) -> (fuel:nat) -> (ins:tainted_ins{let i, _, _ = ins.ops in Mov64? i}) -> (s1:traceState) -> (s2:traceState) -> Lemma
 (let b, ts' = check_if_ins_consumes_fixed_time ins fuel ts in
@@ -446,7 +356,7 @@ let lemma_xor_same_public ts fuel ins s1 s2 =
   let i, dsts, srcs = ins.ops in
   let r1 = taint_eval_ins ins s1 in
   let r2 = taint_eval_ins ins s2 in
-  assert_by_tactic (forall (v:nat64). Types_s.ixor v v = 0) (v <-- forall_intro; apply_lemma (quote lemma_aux_xor));
+  Classical.forall_intro lemma_aux_xor;
   match dsts with
     | [OConst _] -> ()
     | [OReg _] -> ()
@@ -470,7 +380,7 @@ let lemma_xor_same_public ts fuel ins s1 s2 =
 	  assert (b2t b /\ r1.state.ok /\ r2.state.ok /\ publicValuesAreSame ts s1 s2 ==> publicValuesAreSame ts' r1 r2)
 
 #reset-options "--initial_ifuel 2 --max_ifuel 2 --initial_fuel 4 --max_fuel 4 --using_facts_from '* -FStar.Reflection -FStar.Tactics' --z3rlimit 20"
-val lemma_ins_same_public: (ts:taintState) -> (fuel:nat) -> (ins:tainted_ins) -> (s1:traceState) -> (s2:traceState) -> Lemma
+val lemma_ins_same_public: (ts:taintState) -> (fuel:nat) -> (ins:tainted_ins{not (is_xmm_ins ins)}) -> (s1:traceState) -> (s2:traceState) -> Lemma
 (let b, ts' = check_if_ins_consumes_fixed_time ins fuel ts in
   (b2t b ==> isExplicitLeakageFreeGivenStates (Ins ins) fuel ts ts' s1 s2))
 
@@ -488,7 +398,7 @@ let lemma_ins_same_public ts fuel ins s1 s2 = let i, _, _ = ins.ops in
   | Shl64 _ _ -> lemma_shl_same_public ts fuel ins s1 s2
   | Shr64 _ _ -> lemma_shr_same_public ts fuel ins s1 s2
 
-val lemma_ins_leakage_free: (ts:taintState) -> (fuel:nat) -> (ins:tainted_ins) -> Lemma
+val lemma_ins_leakage_free: (ts:taintState) -> (fuel:nat) -> (ins:tainted_ins{not (is_xmm_ins ins)}) -> Lemma
  (let b, ts' = check_if_ins_consumes_fixed_time ins fuel ts in
   (b2t b ==> isConstantTime (Ins ins) fuel ts /\ isLeakageFree (Ins ins) fuel ts ts'))
 
