src/arch/x64/X64.Leakage_Ins_Xmm_i.fst
@@ -1,0 +1,199 @@
+module X64.Leakage_Ins_Xmm_i
+open X64.Machine_s
+open X64.Semantics_s
+open X64.Taint_Semantics_s
+open X64.Leakage_s
+open X64.Leakage_Helpers_i
+open Types_s
+open TypesNative_s
+open FStar.FunctionalExtensionality
+
+let xmm_taint (ts:taintState) (x:xmm) = ts.xmmTaint x
+
+let set_xmm_taint (ts:taintState) (xmm:xmm) (taint:taint) : taintState =
+  TaintState ts.regTaint ts.flagsTaint (fun x -> if x = xmm then taint else ts.xmmTaint x)
+
+#set-options "--z3rlimit 20"
+  
+val quad32_xor_lemma: (x:quad32) -> Lemma (quad32_xor x x == Quad32 0 0 0 0) 
+
+let quad32_xor_lemma x =
+  assert (quad32_xor x x == Quad32 (nat32_xor x.lo x.lo) (nat32_xor x.mid_lo x.mid_lo)
+    (nat32_xor x.mid_hi x.mid_hi) (nat32_xor x.hi x.hi));
+  TypesNative_s.reveal_ixor 32 x.lo x.lo;
+  TypesNative_s.reveal_ixor 32 x.mid_lo x.mid_lo;
+  TypesNative_s.reveal_ixor 32 x.mid_hi x.mid_hi;
+  TypesNative_s.reveal_ixor 32 x.hi x.hi;
+  FStar.UInt.logxor_self #32 x.lo;
+  FStar.UInt.logxor_self #32 x.mid_lo;
+  FStar.UInt.logxor_self #32 x.mid_hi;
+  FStar.UInt.logxor_self #32 x.hi
+
+val check_if_pxor_leakage_free: (ins:tainted_ins{let i, _, _ = ins.ops in Pxor? i}) -> (fuel:nat) -> (ts:taintState) -> (res:(bool*taintState){let b, ts' = res in b2t b ==>
+     isConstantTime (Ins ins) fuel ts /\ isLeakageFree (Ins ins) fuel ts ts'})
+
+let check_if_pxor_leakage_free ins fuel ts =
+  let Pxor dst src, _, _ = ins.ops in
+  if src = dst then begin
+    let ts' = set_xmm_taint ts dst Public in
+    Classical.forall_intro quad32_xor_lemma;
+    true, TaintState ts'.regTaint Secret ts'.xmmTaint
+  end 
+  else begin
+    let taint = merge_taint (xmm_taint ts dst) (xmm_taint ts src) in
+    let ts' = set_xmm_taint ts dst taint in
+    true, TaintState ts'.regTaint Secret ts'.xmmTaint
+  end
+
+val check_if_paddd_leakage_free: (ins:tainted_ins{let i, _, _ = ins.ops in Paddd? i}) -> (fuel:nat) -> (ts:taintState) -> (res:(bool*taintState){let b, ts' = res in b2t b ==>
+     isConstantTime (Ins ins) fuel ts /\ isLeakageFree (Ins ins) fuel ts ts'})
+
+let check_if_paddd_leakage_free ins fuel ts =
+  let Paddd dst src, _, _ = ins.ops in
+  let taint = merge_taint (xmm_taint ts dst) (xmm_taint ts src) in
+  let ts' = set_xmm_taint ts dst taint in
+  true, TaintState ts'.regTaint Secret ts'.xmmTaint
+
+val check_if_pslld_leakage_free: (ins:tainted_ins{let i, _, _ = ins.ops in Pslld? i}) -> (fuel:nat) -> (ts:taintState) -> (res:(bool*taintState){let b, ts' = res in b2t b ==>
+     isConstantTime (Ins ins) fuel ts /\ isLeakageFree (Ins ins) fuel ts ts'})
+
+let check_if_pslld_leakage_free ins fuel ts =
+  let Pslld dst amt, _, _ = ins.ops in
+  let taint = xmm_taint ts dst in
+  let ts' = set_xmm_taint ts dst taint in
+  true, TaintState ts'.regTaint Secret ts'.xmmTaint
+
+val check_if_psrld_leakage_free: (ins:tainted_ins{let i, _, _ = ins.ops in Psrld? i}) -> (fuel:nat) -> (ts:taintState) -> (res:(bool*taintState){let b, ts' = res in b2t b ==>
+     isConstantTime (Ins ins) fuel ts /\ isLeakageFree (Ins ins) fuel ts ts'})
+
+let check_if_psrld_leakage_free ins fuel ts =
+  let Psrld dst amt, _, _ = ins.ops in
+  let taint = xmm_taint ts dst in
+  let ts' = set_xmm_taint ts dst taint in
+  true, TaintState ts'.regTaint Secret ts'.xmmTaint
+
+val check_if_pshufb_leakage_free: (ins:tainted_ins{let i, _, _ = ins.ops in Pshufb? i}) -> (fuel:nat) -> (ts:taintState) -> (res:(bool*taintState){let b, ts' = res in b2t b ==>
+     isConstantTime (Ins ins) fuel ts /\ isLeakageFree (Ins ins) fuel ts ts'})
+
+let check_if_pshufb_leakage_free ins fuel ts =
+  let Pshufb dst src, _, _ = ins.ops in
+  let taint = merge_taint (xmm_taint ts dst) (xmm_taint ts src) in
+  let ts' = set_xmm_taint ts dst taint in
+  true, TaintState ts'.regTaint Secret ts'.xmmTaint
+
+val check_if_pshufd_leakage_free: (ins:tainted_ins{let i, _, _ = ins.ops in Pshufd? i}) -> (fuel:nat) -> (ts:taintState) -> (res:(bool*taintState){let b, ts' = res in b2t b ==>
+     isConstantTime (Ins ins) fuel ts /\ isLeakageFree (Ins ins) fuel ts ts'})
+
+let check_if_pshufd_leakage_free ins fuel ts =
+  let Pshufd dst src _, _, _ = ins.ops in
+  let taint = merge_taint (xmm_taint ts dst) (xmm_taint ts src) in
+  let ts' = set_xmm_taint ts dst taint in
+  true, TaintState ts'.regTaint Secret ts'.xmmTaint
+
+val check_if_pinsrd_leakage_free: (ins:tainted_ins{let i, _, _ = ins.ops in Pinsrd? i}) -> (fuel:nat) -> (ts:taintState) -> (res:(bool*taintState){let b, ts' = res in b2t b ==>
+     isConstantTime (Ins ins) fuel ts /\ isLeakageFree (Ins ins) fuel ts ts'})
+
+let check_if_pinsrd_leakage_free ins fuel ts =
+  let Pinsrd dst src _, _, _ = ins.ops in
+  let fixedTime = operand_does_not_use_secrets src ts in
+  let taint = merge_taint (xmm_taint ts dst) (operand_taint src ts) in
+  let taint = merge_taint taint ins.t in
+  let ts' = set_xmm_taint ts dst taint in
+  fixedTime, TaintState ts'.regTaint Secret ts'.xmmTaint
+
+val check_if_vpslldq_leakage_free: (ins:tainted_ins{let i, _, _ = ins.ops in VPSLLDQ? i}) -> (fuel:nat) -> (ts:taintState) -> (res:(bool*taintState){let b, ts' = res in b2t b ==>
+     isConstantTime (Ins ins) fuel ts /\ isLeakageFree (Ins ins) fuel ts ts'})
+
+let check_if_vpslldq_leakage_free ins fuel ts =
+  let VPSLLDQ dst src _, _, _ = ins.ops in
+  let taint = merge_taint (xmm_taint ts dst) (xmm_taint ts src) in
+  let ts' = set_xmm_taint ts dst taint in
+  true, TaintState ts'.regTaint Secret ts'.xmmTaint
+
+val check_if_pclmuldqd_leakage_free: (ins:tainted_ins{let i, _, _ = ins.ops in Pclmulqdq? i}) -> (fuel:nat) -> (ts:taintState) -> (res:(bool*taintState){let b, ts' = res in b2t b ==>
+     isConstantTime (Ins ins) fuel ts /\ isLeakageFree (Ins ins) fuel ts ts'})
+
+#set-options "--z3rlimit 40"
+
+let check_if_pclmuldqd_leakage_free ins fuel ts =
+  let Pclmulqdq dst src _, _, _ = ins.ops in
+  let taint = merge_taint (xmm_taint ts dst) (xmm_taint ts src) in
+  let ts' = set_xmm_taint ts dst taint in
+  true, TaintState ts'.regTaint Secret ts'.xmmTaint
+
+val check_if_aesni_enc_leakage_free: (ins:tainted_ins{let i, _, _ = ins.ops in AESNI_enc? i}) -> (fuel:nat) -> (ts:taintState) -> (res:(bool*taintState){let b, ts' = res in b2t b ==>
+     isConstantTime (Ins ins) fuel ts /\ isLeakageFree (Ins ins) fuel ts ts'})
+
+let check_if_aesni_enc_leakage_free ins fuel ts =
+  let AESNI_enc dst src, _, _ = ins.ops in
+  let taint = merge_taint (xmm_taint ts dst) (xmm_taint ts src) in
+  let ts' = set_xmm_taint ts dst taint in
+  true, TaintState ts'.regTaint Secret ts'.xmmTaint
+
+val check_if_aesni_enc_last_leakage_free: (ins:tainted_ins{let i, _, _ = ins.ops in AESNI_enc_last? i}) -> (fuel:nat) -> (ts:taintState) -> (res:(bool*taintState){let b, ts' = res in b2t b ==>
+     isConstantTime (Ins ins) fuel ts /\ isLeakageFree (Ins ins) fuel ts ts'})
+
+let check_if_aesni_enc_last_leakage_free ins fuel ts =
+  let AESNI_enc_last dst src, _, _ = ins.ops in
+  let taint = merge_taint (xmm_taint ts dst) (xmm_taint ts src) in
+  let ts' = set_xmm_taint ts dst taint in
+  true, TaintState ts'.regTaint Secret ts'.xmmTaint
+
+val check_if_aesni_dec_leakage_free: (ins:tainted_ins{let i, _, _ = ins.ops in AESNI_dec? i}) -> (fuel:nat) -> (ts:taintState) -> (res:(bool*taintState){let b, ts' = res in b2t b ==>
+     isConstantTime (Ins ins) fuel ts /\ isLeakageFree (Ins ins) fuel ts ts'})
+
+let check_if_aesni_dec_leakage_free ins fuel ts =
+  let AESNI_dec dst src, _, _ = ins.ops in
+  let taint = merge_taint (xmm_taint ts dst) (xmm_taint ts src) in
+  let ts' = set_xmm_taint ts dst taint in
+  true, TaintState ts'.regTaint Secret ts'.xmmTaint
+
+val check_if_aesni_dec_last_leakage_free: (ins:tainted_ins{let i, _, _ = ins.ops in AESNI_dec_last? i}) -> (fuel:nat) -> (ts:taintState) -> (res:(bool*taintState){let b, ts' = res in b2t b ==>
+     isConstantTime (Ins ins) fuel ts /\ isLeakageFree (Ins ins) fuel ts ts'})
+
+let check_if_aesni_dec_last_leakage_free ins fuel ts =
+  let AESNI_dec_last dst src, _, _ = ins.ops in
+  let taint = merge_taint (xmm_taint ts dst) (xmm_taint ts src) in
+  let ts' = set_xmm_taint ts dst taint in
+  true, TaintState ts'.regTaint Secret ts'.xmmTaint
+
+val check_if_aesni_imc_leakage_free: (ins:tainted_ins{let i, _, _ = ins.ops in AESNI_imc? i}) -> (fuel:nat) -> (ts:taintState) -> (res:(bool*taintState){let b, ts' = res in b2t b ==>
+     isConstantTime (Ins ins) fuel ts /\ isLeakageFree (Ins ins) fuel ts ts'})
+
+let check_if_aesni_imc_leakage_free ins fuel ts =
+  let AESNI_imc dst src, _, _ = ins.ops in
+  let taint = merge_taint (xmm_taint ts dst) (xmm_taint ts src) in
+  let ts' = set_xmm_taint ts dst taint in
+  true, TaintState ts'.regTaint Secret ts'.xmmTaint
+
+val check_if_aesni_keygen_leakage_free: (ins:tainted_ins{let i, _, _ = ins.ops in AESNI_keygen_assist? i}) -> (fuel:nat) -> (ts:taintState) -> (res:(bool*taintState){let b, ts' = res in b2t b ==>
+     isConstantTime (Ins ins) fuel ts /\ isLeakageFree (Ins ins) fuel ts ts'})
+
+let check_if_aesni_keygen_leakage_free ins fuel ts =
+  let AESNI_keygen_assist dst src _, _, _ = ins.ops in
+  let taint = merge_taint (xmm_taint ts dst) (xmm_taint ts src) in
+  let ts' = set_xmm_taint ts dst taint in
+  true, TaintState ts'.regTaint Secret ts'.xmmTaint
+
+val check_if_xmm_ins_consumes_fixed_time: (ins:tainted_ins{is_xmm_ins ins}) -> (fuel:nat) -> (ts:taintState) -> (res:(bool*taintState){ins_consumes_fixed_time ins fuel ts res})
+
+let check_if_xmm_ins_consumes_fixed_time ins fuel ts =
+  let i, _, _ = ins.ops in
+  match i with
+    | Paddd dst src -> check_if_paddd_leakage_free ins fuel ts
+    | Pxor dst src -> check_if_pxor_leakage_free ins fuel ts
+    | Pslld dst amt -> check_if_pslld_leakage_free ins fuel ts
+    | Psrld dst amt -> check_if_psrld_leakage_free ins fuel ts
+    | Pshufb dst src -> check_if_pshufb_leakage_free ins fuel ts
+    | Pshufd dst src permutation -> check_if_pshufd_leakage_free ins fuel ts
+    | Pinsrd dst srx index -> check_if_pinsrd_leakage_free ins fuel ts
+    | VPSLLDQ dst src count -> check_if_vpslldq_leakage_free ins fuel ts
+    | MOVDQU dst src -> false, ts
+    | Pclmulqdq dst src imm -> check_if_pclmuldqd_leakage_free ins fuel ts
+    | AESNI_enc dst src -> check_if_aesni_enc_leakage_free ins fuel ts
+    | AESNI_enc_last dst src -> check_if_aesni_enc_last_leakage_free ins fuel ts
+    | AESNI_dec dst src -> check_if_aesni_dec_leakage_free ins fuel ts
+    | AESNI_dec_last dst src -> check_if_aesni_dec_last_leakage_free ins fuel ts
+    | AESNI_imc dst src -> check_if_aesni_imc_leakage_free ins fuel ts
+    | AESNI_keygen_assist dst src imm -> check_if_aesni_keygen_leakage_free ins fuel ts
+    
