SConscript
@@ -98,6 +98,7 @@ verify_options = {
   'src/arch/x64/X64.Taint_Semantics_s.fst': None,
   'src/arch/x64/X64.Leakage_s.fst': None,
   'src/arch/x64/X64.Leakage_Ins_i.fst': None,
+  'src/arch/x64/X64.Leakage_Ins_Xmm_i.fst': None,
   'src/arch/x64/X64.Leakage_i.fst': None,
   'src/arch/x64/X64.Leakage_Helpers_i.fst': None,
   'tools/Vale/test/vale-debug.vad': None,
